proof/invariant-abstract/RISCV64/ArchIpc_AI.thy
@@ -218,21 +218,17 @@ lemma copy_mrs_in_user_frame[wp, Ipc_AI_2_assms]:
   "\<lbrace>in_user_frame p\<rbrace> copy_mrs t buf t' buf' n \<lbrace>\<lambda>rv. in_user_frame p\<rbrace>"
   by (simp add: in_user_frame_def) (wp hoare_vcg_ex_lift)
 
-lemma as_user_getRestart_invs[wp]: "\<lbrace>P\<rbrace> as_user t getRestartPC \<lbrace>\<lambda>_. P\<rbrace>"
+lemma as_user_getRestart_inv[wp]:
+  "as_user t getRestartPC \<lbrace>P\<rbrace>"
   by (simp add: getRestartPC_def, rule user_getreg_inv)
 
-lemma make_arch_fault_msg_invs[wp, Ipc_AI_2_assms]: "make_arch_fault_msg f t \<lbrace>invs\<rbrace>"
-  by (cases f; wpsimp)
+lemma make_arch_fault_msg_inv[wp, Ipc_AI_2_assms]:
+  "make_arch_fault_msg ft t \<lbrace>P\<rbrace>"
+  by (cases ft; wpsimp)
 
-lemma make_fault_message_inv[wp, Ipc_AI_2_assms]:
-  "make_fault_msg ft t \<lbrace>invs\<rbrace>"
-  apply (cases ft, simp_all split del: if_split)
-     apply (wp as_user_inv getRestartPC_inv mapM_wp'
-              | simp add: getRegister_def)+
-  done
-
-crunch make_fault_msg
-  for tcb_at[wp]: "tcb_at t"
+lemma make_fault_msg_inv[wp, Ipc_AI_2_assms]:
+  "make_fault_msg ft t \<lbrace>P\<rbrace>"
+  by (cases ft; wpsimp wp: as_user_inv getRestartPC_inv mapM_wp' split_del: if_split)
 
 lemma do_fault_transfer_invs[wp, Ipc_AI_2_assms]:
   "\<lbrace>invs and tcb_at receiver\<rbrace>
@@ -496,7 +492,7 @@ lemma setup_caller_cap_aobj_at:
 
 lemma setup_caller_cap_valid_arch[Ipc_AI_2_assms, wp]:
   "setup_caller_cap st rt grant \<lbrace>valid_arch_state\<rbrace>"
-  by (wpsimp wp: valid_arch_state_lift_aobj_at_no_caps[rotated -1] setup_caller_cap_aobj_at)
+  by (wpsimp wp: valid_arch_state_lift_aobj_at_no_caps[rotated -1] setup_caller_cap_tcb_at setup_caller_cap_aobj_at)
 
 lemma transfer_caps_loop_valid_arch[Ipc_AI_2_assms]:
   "\<And>slots caps ep buffer n mi.
@@ -505,7 +501,7 @@ lemma transfer_caps_loop_valid_arch[Ipc_AI_2_assms]:
          and transfer_caps_srcs caps\<rbrace>
       transfer_caps_loop ep buffer n caps slots mi
     \<lbrace>\<lambda>_. valid_arch_state\<rbrace>"
-  by (wpsimp wp: valid_arch_state_lift_aobj_at_no_caps transfer_caps_loop_aobj_at)
+  by (wpsimp wp: valid_arch_state_lift_aobj_at_no_caps transfer_caps_loop_typ_ats transfer_caps_loop_aobj_at)
 
 end
 
@@ -570,7 +566,7 @@ lemma do_ipc_transfer_valid_arch[Ipc_AI_3_assms]:
   "\<lbrace>valid_arch_state and valid_objs and valid_mdb \<rbrace>
    do_ipc_transfer s ep bg grt r
    \<lbrace>\<lambda>rv. valid_arch_state\<rbrace>"
-  by (wpsimp wp: valid_arch_state_lift_aobj_at_no_caps do_ipc_transfer_aobj_at)
+  by (wpsimp wp: valid_arch_state_lift_aobj_at_no_caps dit_tcb_at do_ipc_transfer_aobj_at)
 
 end
 
